src/guarding/lib/boxes.v
@@ -1,0 +1,444 @@
+(* This is a modified version of iris/iris/basic_logic/lib/boxes.v
+and is distributed under the Iris license:
+
+All files in this development, excluding those in docs/ and tex/, are
+distributed under the terms of the 3-clause BSD license
+(https://opensource.org/licenses/BSD-3-Clause), included below.
+
+Copyright: Iris developers and contributors
+
+------------------------------------------------------------------------------
+
+Redistribution and use in source and binary forms, with or without
+modification, are permitted provided that the following conditions are met:
+    * Redistributions of source code must retain the above copyright
+      notice, this list of conditions and the following disclaimer.
+    * Redistributions in binary form must reproduce the above copyright
+      notice, this list of conditions and the following disclaimer in the
+      documentation and/or other materials provided with the distribution.
+    * Neither the name of the copyright holder nor the names of its contributors
+      may be used to endorse or promote products derived from this software
+      without specific prior written permission.
+
+THIS SOFTWARE IS PROVIDED BY THE COPYRIGHT HOLDERS AND CONTRIBUTORS "AS IS" AND
+ANY EXPRESS OR IMPLIED WARRANTIES, INCLUDING, BUT NOT LIMITED TO, THE IMPLIED
+WARRANTIES OF MERCHANTABILITY AND FITNESS FOR A PARTICULAR PURPOSE ARE
+DISCLAIMED. IN NO EVENT SHALL THE COPYRIGHT HOLDER OR CONTRIBUTORS BE LIABLE FOR
+ANY DIRECT, INDIRECT, INCIDENTAL, SPECIAL, EXEMPLARY, OR CONSEQUENTIAL DAMAGES
+(INCLUDING, BUT NOT LIMITED TO, PROCUREMENT OF SUBSTITUTE GOODS OR SERVICES;
+LOSS OF USE, DATA, OR PROFITS; OR BUSINESS INTERRUPTION) HOWEVER CAUSED AND ON
+ANY THEORY OF LIABILITY, WHETHER IN CONTRACT, STRICT LIABILITY, OR TORT
+(INCLUDING NEGLIGENCE OR OTHERWISE) ARISING IN ANY WAY OUT OF THE USE OF THIS
+SOFTWARE, EVEN IF ADVISED OF THE POSSIBILITY OF SUCH DAMAGE.
+*)
+
+(** This is an extension of the Iris "boxes" library.
+See the Iris appendix for an introduction to what boxes are: https://plv.mpi-sws.org/iris/appendix-4.3.pdf
+
+All the standard Box logical rules are unmodified. The only difference is that this version
+of the boxes library now provides additional guard properties.
+
+The model of boxes is almost exactly the same, except we need to use the
+Leaf-style invariants ([True &&{↑N}&&> ▷ Q]) instead of normal Iris invariants ([inv N Q]).
+However, all the public-facing rules are the same.
+*)
+
+From iris.algebra Require Import lib.excl_auth gmap agree.
+From iris.proofmode Require Import proofmode.
+From iris.base_logic.lib Require Export invariants.
+From iris.prelude Require Import options.
+Import uPred.
+
+Require Import guarding.guard.
+Require Import guarding.tactics.
+Require Import guarding.own_and.
+Require Import guarding.internal.auth_frag_util.
+
+(** The CMRAs we need. *)
+Class boxG Σ :=
+  #[local] boxG_inG :: inG Σ (prodR
+    (excl_authR boolO)
+    (optionR (agreeR (laterO (iPropO Σ))))).
+
+Definition boxΣ : gFunctors := #[ GFunctor (excl_authR boolO *
+                                            optionRF (agreeRF (▶ ∙)) ) ].
+
+Global Instance subG_boxΣ Σ : subG boxΣ Σ → boxG Σ.
+Proof. solve_inG. Qed.
+
+(** Standard boxes interface *)
+
+Section box_defs.
+  Context `{!invGS_gen hlc Σ, !boxG Σ} (N : namespace).
+
+  Definition slice_name := gname.
+
+  Definition box_own_auth (γ : slice_name) (a : excl_authR boolO) : iProp Σ :=
+    own γ (a, None).
+
+  Definition box_own_prop (γ : slice_name) (P : iProp Σ) : iProp Σ :=
+    own γ (ε, Some (to_agree (Next P))).
+
+  Definition slice_inv (γ : slice_name) (P : iProp Σ) : iProp Σ :=
+    ∃ b, box_own_auth γ (●E b) ∗ if b then P else True.
+
+  Definition slice (γ : slice_name) (P : iProp Σ) : iProp Σ :=
+    box_own_prop γ P ∗ (True &&{↑N}&&> ▷ (slice_inv γ P)).
+
+  Definition box (f : gmap slice_name bool) (P : iProp Σ) : iProp Σ :=
+    tc_opaque (∃ Φ : slice_name → iProp Σ,
+      ▷ (P ≡ [∗ map] γ ↦ _ ∈ f, Φ γ) ∗
+      [∗ map] γ ↦ b ∈ f, box_own_auth γ (◯E b) ∗ box_own_prop γ (Φ γ) ∗
+                         (True &&{↑N}&&> ▷ (slice_inv γ (Φ γ))))%I.
+End box_defs.
+
+Global Instance: Params (@box_own_prop) 3 := {}.
+Global Instance: Params (@slice_inv) 3 := {}.
+Global Instance: Params (@slice) 5 := {}.
+Global Instance: Params (@box) 5 := {}.
+
+Section box.
+Context `{!invGS_gen hlc Σ, !boxG Σ} (N : namespace).
+Implicit Types P Q : iProp Σ.
+
+Global Instance box_own_prop_ne γ : NonExpansive (box_own_prop γ).
+Proof. solve_proper. Qed.
+Global Instance box_own_prop_contractive γ : Contractive (box_own_prop γ).
+Proof. solve_contractive. Qed.
+
+Global Instance box_inv_ne γ : NonExpansive (slice_inv γ).
+Proof. solve_proper. Qed.
+
+Global Instance slice_ne γ : NonExpansive (slice N γ).
+Proof. solve_proper. Qed.
+Global Instance slice_contractive γ : Contractive (slice N γ).
+Proof. solve_contractive. Qed.
+Global Instance slice_proper γ : Proper ((≡) ==> (≡)) (slice N γ).
+Proof. apply ne_proper, _. Qed.
+
+Global Instance slice_persistent γ P : Persistent (slice N γ P).
+Proof. apply _. Qed.
+
+Global Instance box_contractive f : Contractive (box N f).
+Proof. solve_contractive. Qed.
+Global Instance box_ne f : NonExpansive (box N f).
+Proof. apply (contractive_ne _). Qed.
+Global Instance box_proper f : Proper ((≡) ==> (≡)) (box N f).
+Proof. apply ne_proper, _. Qed.
+
+Lemma box_own_auth_agree γ b1 b2 :
+  box_own_auth γ (●E b1) ∗ box_own_auth γ (◯E b2) ⊢ ⌜b1 = b2⌝.
+Proof.
+  rewrite /box_own_prop -own_op own_valid prod_validI /= and_elim_l.
+  by iDestruct 1 as %?%excl_auth_agree_L.
+Qed.
+
+Lemma box_own_auth_update γ b1 b2 b3 :
+  box_own_auth γ (●E b1) ∗ box_own_auth γ (◯E b2)
+  ==∗ box_own_auth γ (●E b3) ∗ box_own_auth γ (◯E b3).
+Proof.
+  rewrite /box_own_auth -!own_op. iApply own_update. apply prod_update; last done.
+  apply excl_auth_update.
+Qed.
+
+Lemma box_own_agree γ Q1 Q2 :
+  box_own_prop γ Q1 ∗ box_own_prop γ Q2 ⊢ ▷ (Q1 ≡ Q2).
+Proof.
+  rewrite /box_own_prop -own_op own_valid prod_validI /= and_elim_r.
+  by rewrite option_validI /= agree_validI agree_equivI later_equivI /=.
+Qed.
+
+Lemma box_alloc : ⊢ box N ∅ True.
+Proof.
+  iIntros. iExists (λ _, True)%I. by rewrite !big_opM_empty.
+Qed.
+
+Lemma slice_insert_empty E q f Q P :
+  ▷?q box N f P ={E}=∗ ∃ γ, ⌜f !! γ = None⌝ ∗
+    slice N γ Q ∗ ▷?q box N (<[γ:=false]> f) (Q ∗ P).
+Proof.
+  iDestruct 1 as (Φ) "[#HeqP Hf]".
+  iMod (own_alloc_cofinite (●E false ⋅ ◯E false,
+    Some (to_agree (Next Q))) (dom f))
+    as (γ) "[Hdom Hγ]"; first by (split; [apply auth_both_valid_discrete|]).
+  rewrite pair_split. iDestruct "Hγ" as "[[Hγ Hγ'] #HγQ]".
+  iDestruct "Hdom" as % ?%not_elem_of_dom.
+  iMod (guards_alloc _ N (slice_inv γ Q) with "[Hγ]") as "#Hinv".
+  { iNext. iExists false; eauto. }
+  iModIntro; iExists γ; repeat iSplit; auto.
+  iNext. iExists (<[γ:=Q]> Φ); iSplit.
+  - iNext. iRewrite "HeqP". by rewrite big_opM_fn_insert'.
+  - rewrite (big_opM_fn_insert (λ _ _ P',  _ ∗ _ _ P' ∗ _ _ _ _ (_ (_ _ P'))))%I //.
+    iFrame; eauto.
+Qed.
+
+Lemma slice_delete_empty E q f P Q γ :
+  ↑N ⊆ E →
+  f !! γ = Some false →
+  slice N γ Q -∗ ▷?q box N f P ={E}=∗ ∃ P',
+    ▷?q (▷ (P ≡ (Q ∗ P')) ∗ box N (delete γ f) P').
+Proof.
+  iIntros (??) "[#HγQ Hguards] H". iDestruct "H" as (Φ) "[#HeqP Hf]".
+  iExists ([∗ map] γ'↦_ ∈ delete γ f, Φ γ')%I.
+  iDestruct (inv_from_guards with "Hguards") as "Hinv".
+  iInv N as (b) "[>Hγ _]".
+  iDestruct (big_sepM_delete _ f _ false with "Hf")
+    as "[[>Hγ' #[HγΦ ?]] ?]"; first done.
+  iDestruct (box_own_auth_agree γ b false with "[-]") as %->; first by iFrame.
+  iModIntro. iSplitL "Hγ"; first iExists false; eauto.
+  iModIntro. iNext. iSplit.
+  - iDestruct (box_own_agree γ Q (Φ γ) with "[#]") as "HeqQ"; first by eauto.
+    iNext. iRewrite "HeqP". iRewrite "HeqQ". by rewrite -big_opM_delete.
+  - iExists Φ; eauto.
+Qed.
+
+Lemma slice_fill E q f γ P Q :
+  ↑N ⊆ E →
+  f !! γ = Some false →
+  slice N γ Q -∗ ▷ Q -∗ ▷?q box N f P ={E}=∗ ▷?q box N (<[γ:=true]> f) P.
+Proof.
+  iIntros (??) "#[HγQ Hguards] HQ H"; iDestruct "H" as (Φ) "[#HeqP Hf]".
+  iDestruct (inv_from_guards with "Hguards") as "Hinv".
+  iInv N as (b') "[>Hγ _]".
+  iDestruct (big_sepM_delete _ f _ false with "Hf")
+    as "[[>Hγ' #[HγΦ Hinv']] ?]"; first done.
+  iMod (box_own_auth_update γ b' false true with "[$Hγ $Hγ']") as "[Hγ Hγ']".
+  iModIntro. iSplitL "Hγ HQ"; first (iNext; iExists true; by iFrame).
+  iModIntro; iNext; iExists Φ; iSplit.
+  - by rewrite big_opM_insert_override.
+  - rewrite -insert_delete_insert big_opM_insert ?lookup_delete //.
+    iFrame; eauto.
+Qed.
+
+Lemma slice_empty E q f P Q γ :
+  ↑N ⊆ E →
+  f !! γ = Some true →
+  slice N γ Q -∗ ▷?q box N f P ={E}=∗ ▷ Q ∗ ▷?q box N (<[γ:=false]> f) P.
+Proof.
+  iIntros (??) "#[HγQ Hguards] H"; iDestruct "H" as (Φ) "[#HeqP Hf]".
+  iDestruct (inv_from_guards with "Hguards") as "Hinv".
+  iInv N as (b) "[>Hγ HQ]".
+  iDestruct (big_sepM_delete _ f with "Hf")
+    as "[[>Hγ' #[HγΦ Hinv']] ?]"; first done.
+  iDestruct (box_own_auth_agree γ b true with "[-]") as %->; first by iFrame.
+  iFrame "HQ".
+  iMod (box_own_auth_update γ with "[$Hγ $Hγ']") as "[Hγ Hγ']".
+  iModIntro. iSplitL "Hγ"; first (iNext; iExists false; by repeat iSplit).
+  iModIntro; iNext; iExists Φ; iSplit.
+  - by rewrite big_opM_insert_override.
+  - rewrite -insert_delete_insert big_opM_insert ?lookup_delete //.
+    iFrame; eauto.
+Qed.
+
+Lemma slice_insert_full E q f P Q :
+  ↑N ⊆ E →
+  ▷ Q -∗ ▷?q box N f P ={E}=∗ ∃ γ, ⌜f !! γ = None⌝ ∗
+    slice N γ Q ∗ ▷?q box N (<[γ:=true]> f) (Q ∗ P).
+Proof.
+  iIntros (?) "HQ Hbox".
+  iMod (slice_insert_empty with "Hbox") as (γ ?) "[#Hslice Hbox]".
+  iExists γ. iFrame "%#". iMod (slice_fill with "Hslice HQ Hbox"); first done.
+  - by apply lookup_insert.
+  - by rewrite insert_insert.
+Qed.
+
+Lemma slice_delete_full E q f P Q γ :
+  ↑N ⊆ E →
+  f !! γ = Some true →
+  slice N γ Q -∗ ▷?q box N f P ={E}=∗
+  ∃ P', ▷ Q ∗ ▷?q ▷ (P ≡ (Q ∗ P')) ∗ ▷?q box N (delete γ f) P'.
+Proof.
+  iIntros (??) "#Hslice Hbox".
+  iMod (slice_empty with "Hslice Hbox") as "[$ Hbox]"; try done.
+  iMod (slice_delete_empty with "Hslice Hbox") as (P') "[Heq Hbox]"; first done.
+  { by apply lookup_insert. }
+  iExists P'. iFrame. rewrite -insert_delete_insert delete_insert ?lookup_delete //.
+Qed.
+
+Lemma box_fill E f P :
+  ↑N ⊆ E →
+  box N f P -∗ ▷ P ={E}=∗ box N (const true <$> f) P.
+Proof.
+  iIntros (?) "H HP"; iDestruct "H" as (Φ) "[#HeqP Hf]".
+  iExists Φ; iSplitR; first by rewrite big_opM_fmap.
+  iEval (rewrite internal_eq_iff later_iff big_sepM_later) in "HeqP".
+  iDestruct ("HeqP" with "HP") as "HP".
+  iCombine "Hf" "HP" as "Hf".
+  rewrite -big_sepM_sep big_opM_fmap; iApply (big_sepM_fupd _ _ f).
+  iApply (@big_sepM_impl with "Hf").
+  iIntros "!>" (γ b' ?) "[(Hγ' & #$ & #Hguards) HΦ]".
+  iDestruct (inv_from_guards with "Hguards") as "Hinv".
+  iInv N as (b) "[>Hγ _]".
+  iMod (box_own_auth_update γ with "[Hγ Hγ']") as "[Hγ $]"; first by iFrame.
+  iModIntro. iSplitL; last done. iNext; iExists true. iFrame.
+Qed.
+
+Lemma box_empty E f P :
+  ↑N ⊆ E →
+  map_Forall (λ _, (true =.)) f →
+  box N f P ={E}=∗ ▷ P ∗ box N (const false <$> f) P.
+Proof.
+  iDestruct 1 as (Φ) "[#HeqP Hf]".
+  iAssert (([∗ map] γ↦b ∈ f, ▷ Φ γ) ∗
+    [∗ map] γ↦b ∈ f, box_own_auth γ (◯E false) ∗  box_own_prop γ (Φ γ) ∗
+      (True &&{↑N}&&> ▷ (slice_inv γ (Φ γ))))%I with "[> Hf]" as "[HΦ ?]".
+  { rewrite -big_sepM_sep -big_sepM_fupd. iApply (@big_sepM_impl with "[$Hf]").
+    iIntros "!>" (γ b ?) "(Hγ' & #HγΦ & #Hguards)".
+    iDestruct (inv_from_guards with "Hguards") as "Hinv".
+    assert (true = b) as <- by eauto.
+    iInv N as (b) "[>Hγ HΦ]".
+    iDestruct (box_own_auth_agree γ b true with "[-]") as %->; first by iFrame.
+    iMod (box_own_auth_update γ true true false with "[$Hγ $Hγ']") as "[Hγ $]".
+    iModIntro. iSplitL "Hγ"; first (iNext; iExists false; iFrame; eauto).
+    iFrame "HγΦ Hguards". by iApply "HΦ". }
+  iModIntro; iSplitL "HΦ".
+  - rewrite internal_eq_iff later_iff big_sepM_later. by iApply "HeqP".
+  - iExists Φ; iSplit; by rewrite big_opM_fmap.
+Qed.
+
+Lemma slice_iff E q f P Q Q' γ b :
+  ↑N ⊆ E → f !! γ = Some b →
+  ▷ □ (Q ↔ Q') -∗ slice N γ Q -∗ ▷?q box N f P ={E}=∗ ∃ γ' P',
+    ⌜delete γ f !! γ' = None⌝ ∗ ▷?q ▷ □ (P ↔ P') ∗
+    slice N γ' Q' ∗ ▷?q box N (<[γ' := b]>(delete γ f)) P'.
+Proof.
+  iIntros (??) "#HQQ' #Hs Hb". destruct b.
+  - iMod (slice_delete_full with "Hs Hb") as (P') "(HQ & Heq & Hb)"; try done.
+    iDestruct ("HQQ'" with "HQ") as "HQ'".
+    iMod (slice_insert_full with "HQ' Hb") as (γ' ?) "[#Hs' Hb]"; try done.
+    iExists γ', _. iIntros "{$∗ $# $%} !>". do 2 iNext. iRewrite "Heq".
+    iIntros "!>". by iSplit; iIntros "[? $]"; iApply "HQQ'".
+  - iMod (slice_delete_empty with "Hs Hb") as (P') "(Heq & Hb)"; try done.
+    iMod (slice_insert_empty with "Hb") as (γ' ?) "[#Hs' Hb]"; try done.
+    iExists γ', (Q' ∗ P')%I. iIntros "{$∗ $# $%} !>".  do 2 iNext. iRewrite "Heq".
+    iIntros "!>". by iSplit; iIntros "[? $]"; iApply "HQQ'".
+Qed.
+
+Lemma slice_split E q f P Q1 Q2 γ b :
+  ↑N ⊆ E → f !! γ = Some b →
+  slice N γ (Q1 ∗ Q2) -∗ ▷?q box N f P ={E}=∗ ∃ γ1 γ2,
+    ⌜delete γ f !! γ1 = None⌝ ∗ ⌜delete γ f !! γ2 = None⌝ ∗ ⌜γ1 ≠ γ2⌝ ∗
+    slice N γ1 Q1 ∗ slice N γ2 Q2 ∗ ▷?q box N (<[γ2 := b]>(<[γ1 := b]>(delete γ f))) P.
+Proof.
+  iIntros (??) "#Hslice Hbox". destruct b.
+  - iMod (slice_delete_full with "Hslice Hbox") as (P') "([HQ1 HQ2] & Heq & Hbox)"; try done.
+    iMod (slice_insert_full with "HQ1 Hbox") as (γ1 ?) "[#Hslice1 Hbox]"; first done.
+    iMod (slice_insert_full with "HQ2 Hbox") as (γ2 ?) "[#Hslice2 Hbox]"; first done.
+    iExists γ1, γ2. iIntros "{$% $#} !>". iSplit; last iSplit; try iPureIntro.
+    { by eapply lookup_insert_None. }
+    { by apply (lookup_insert_None (delete γ f) γ1 γ2 true). }
+    iNext. iApply (internal_eq_rewrite_contractive _ _ (box _ _) with "[Heq] Hbox").
+    iNext. iRewrite "Heq". iPureIntro. by rewrite assoc (comm _ Q2).
+  - iMod (slice_delete_empty with "Hslice Hbox") as (P') "[Heq Hbox]"; try done.
+    iMod (slice_insert_empty with "Hbox") as (γ1 ?) "[#Hslice1 Hbox]".
+    iMod (slice_insert_empty with "Hbox") as (γ2 ?) "[#Hslice2 Hbox]".
+    iExists γ1, γ2. iIntros "{$% $#} !>". iSplit; last iSplit; try iPureIntro.
+    { by eapply lookup_insert_None. }
+    { by apply (lookup_insert_None (delete γ f) γ1 γ2 false). }
+    iNext. iApply (internal_eq_rewrite_contractive _ _ (box _ _) with "[Heq] Hbox").
+    iNext. iRewrite "Heq". iPureIntro. by rewrite assoc (comm _ Q2).
+Qed.
+
+Lemma slice_combine E q f P Q1 Q2 γ1 γ2 b :
+  ↑N ⊆ E → γ1 ≠ γ2 → f !! γ1 = Some b → f !! γ2 = Some b →
+  slice N γ1 Q1 -∗ slice N γ2 Q2 -∗ ▷?q box N f P ={E}=∗ ∃ γ,
+    ⌜delete γ2 (delete γ1 f) !! γ = None⌝ ∗ slice N γ (Q1 ∗ Q2) ∗
+    ▷?q box N (<[γ := b]>(delete γ2 (delete γ1 f))) P.
+Proof.
+  iIntros (????) "#Hslice1 #Hslice2 Hbox". destruct b.
+  - iMod (slice_delete_full with "Hslice1 Hbox") as (P1) "(HQ1 & Heq1 & Hbox)"; try done.
+    iMod (slice_delete_full with "Hslice2 Hbox") as (P2) "(HQ2 & Heq2 & Hbox)"; first done.
+    { by simplify_map_eq. }
+    iMod (slice_insert_full _ _ _ _ (Q1 ∗ Q2) with "[$HQ1 $HQ2] Hbox")
+      as (γ ?) "[#Hslice Hbox]"; first done.
+    iExists γ. iIntros "{$% $#} !>". iNext.
+    iApply (internal_eq_rewrite_contractive _ _ (box _ _) with "[Heq1 Heq2] Hbox").
+    iNext. iRewrite "Heq1". iRewrite "Heq2". by rewrite assoc.
+  - iMod (slice_delete_empty with "Hslice1 Hbox") as (P1) "(Heq1 & Hbox)"; try done.
+    iMod (slice_delete_empty with "Hslice2 Hbox") as (P2) "(Heq2 & Hbox)"; first done.
+    { by simplify_map_eq. }
+    iMod (slice_insert_empty with "Hbox") as (γ ?) "[#Hslice Hbox]".
+    iExists γ. iIntros "{$% $#} !>". iNext.
+    iApply (internal_eq_rewrite_contractive _ _ (box _ _) with "[Heq1 Heq2] Hbox").
+    iNext. iRewrite "Heq1". iRewrite "Heq2". by rewrite assoc.
+Qed.
+
+(** New Leaf-specific rules *)
+
+(* begin hide *)
+Local Lemma incl_pair_L (a1 a2 : excl_authR boolO) (o1 o2 : optionR (agreeR (laterO (iPropO Σ))))
+    : @uPred_cmra_incl Σ _ (Some (a1, o1)) (Some (a2, o2)) ⊢ ⌜a1 ≼ a2⌝.
+Proof.
+  iIntros "H". iDestruct "H" as (t) "H". destruct t as [[x y]|].
+    - setoid_rewrite <- Some_op.
+      setoid_rewrite option_equivI.
+      setoid_rewrite <- pair_op.
+      setoid_rewrite prod_equivI. simpl. iDestruct "H" as "[H _]".
+      iDestruct (discrete_eq_1 with "H") as "%H".
+      iPureIntro. exists x. trivial.
+    - setoid_rewrite op_None_right_id.
+      setoid_rewrite option_equivI.
+      setoid_rewrite prod_equivI. simpl. iDestruct "H" as "[H _]".
+      iDestruct (discrete_eq_1 with "H") as "%H".
+      iPureIntro. exists ε. rewrite right_id. apply H.
+Qed.
+
+Local Lemma box_own_auth_agree_and γ b1 b2 o1 o2
+  : own γ (◯E b1, o1) ∧ own γ (●E b2, o2) ⊢ ⌜ b1 = b2 ⌝.
+Proof using N boxG0 hlc invGS_gen0 Σ.
+  iIntros "X". iDestruct (and_own with "X") as (z) "[H [Hincl1 Hincl2]]".
+  
+  iDestruct (own_valid with "H") as "#Hval". destruct z as [au o].
+  rewrite prod_validI. simpl. iDestruct "Hval" as "[%Hval _]".
+  
+  iDestruct (incl_pair_L with "Hincl1") as "%Hincl1".
+  iDestruct (incl_pair_L with "Hincl2") as "%Hincl2".
+  
+  iPureIntro.
+  assert (Excl' b1 ≼ Excl' b2) as X.
+   { apply (@auth_frag_incl (optionUR (exclR boolO)) (option_cmra_discrete _) _ _ _ Hincl2 Hincl1 Hval). }
+  rewrite Excl_included in X. apply X.
+Qed.
+(* end hide *)
+
+Lemma box_guard f P Q γ :
+    f !! γ = Some true →
+    slice N γ Q ⊢ box N f P &&{↑N}&&> ▷ Q.
+Proof.
+  intros Hfull. unfold slice. iIntros "[#Hbox #Hguards]".
+  rewrite bi.later_exist.
+  
+  simpl.
+  unfold slice_inv.
+  leaf_hyp "Hguards" lhs to (box N f P) as "Hguards1".
+  { iApply guards_true. }
+  iDestruct (guards_strengthen_exists_with_lhs _ _ (λ b , ▷ ⌜b = true⌝)%I with "Hguards1")
+      as "Hguards2".
+  { intros x. iIntros "H". iNext.
+    iAssert (box_own_auth γ (◯E true) ∧ box_own_auth γ (●E x))%I with "[H]" as "H".
+    {
+      iSplit.
+      {
+        iDestruct "H" as "[H _]".
+        iDestruct "H" as (Φ) "[_ Hmap]".
+        rewrite (big_sepM_delete _ f γ true Hfull).
+        iDestruct "Hmap" as "[[H _] _]".
+        iFrame.
+      }
+      { iDestruct "H" as "[_ [H J]]". iFrame. }
+    }
+    unfold box_own_auth.
+    iDestruct (box_own_auth_agree_and with "H") as "%H". iPureIntro.
+    symmetry. trivial.
+  }
+  leaf_hyp "Hguards2" rhs to (▷ Q)%I as "Hguards3".
+  - leaf_by_sep_except0.
+    iIntros "H". iDestruct "H" as (b) "[H Hbtrue]". iMod "Hbtrue" as "%Hbtrue".
+    subst b. iDestruct "H" as "[H J]". iModIntro. iFrame "J". iIntros "J".
+    iExists true. iFrame. iModIntro. iPureIntro. trivial.
+  - iFrame "Hguards3".
+Qed.
+
+End box.
+
+Global Typeclasses Opaque slice box.
